Can't prove it

DVE.v
@@ -2,15 +2,15 @@ Require Import CSet Le.
 Require Import Plus Util AllInRel Map.
 
 Require Import Val EqDec Computable Var Env EnvTy IL Annotation.
-Require Import Sim Fresh Filter Liveness TrueLiveness Filter MoreExp.
+Require Import Sim Fresh Filter Liveness TrueLiveness Filter MoreExp OUnion.
 
 Set Implicit Arguments.
 Unset Printing Records.
 
-Fixpoint compile (LV:list (set var * params)) (s:stmt) (a:ann (set var)) :=
+Fixpoint compile (LV:list (؟ (set var) * params)) (s:stmt) (a:ann (؟(set var))) :=
   match s, a with
     | stmtLet x e s, ann1 lv an =>
-      if [x ∈ getAnn an] then stmtLet x e (compile LV s an)
+      if [x ∈ getOAnn an] then stmtLet x e (compile LV s an)
                          else compile LV s an
     | stmtIf e s t, ann2 _ ans ant =>
       if [exp2bool e = Some true] then
@@ -20,188 +20,255 @@ Fixpoint compile (LV:list (set var * params)) (s:stmt) (a:ann (set var)) :=
       else
         stmtIf e (compile LV s ans) (compile LV t ant)
     | stmtApp f Y, ann0 lv =>
-      let lvZ := nth (counted f) LV (∅,nil) in
-      stmtApp f (filter_by (fun y => B[y ∈ fst lvZ]) (snd lvZ) Y)
+      let lvZ := nth (counted f) LV (None, nil) in
+      stmtApp f (filter_by (fun y => B[y ∈ oget (fst lvZ)]) (snd lvZ) Y)
     | stmtReturn x, ann0 _ => stmtReturn x
     | stmtExtern x f e s, ann1 lv an =>
       stmtExtern x f e (compile LV s an)
     | stmtFun F t, annF lv ans ant =>
       let LV' := pair ⊜ (getAnn ⊝ ans) (fst ⊝ F) ++ LV in
-      stmtFun (zip (fun Zs a => (List.filter (fun x => B[x ∈ getAnn a]) (fst Zs),
+      stmtFun (zip (fun Zs a => (List.filter (fun x => B[x ∈ getOAnn a]) (fst Zs),
                               compile LV' (snd Zs) a)) F ans)
               (compile LV' t ant)
     | s, _ => s
   end.
 
-Definition ArgRel (V V:onv val) (G:(set var * params)) (VL VL': list val) : Prop :=
-  VL' = (filter_by (fun x => B[x ∈ (fst G)]) (snd G) VL) /\
-  length (snd G) = length VL.
 
-Definition ParamRel (G:(set var * params)) (Z Z' : list var) : Prop :=
-  Z' = (List.filter (fun x => B[x ∈ (fst G)]) Z) /\ snd G = Z.
-
-Instance SR : ProofRelation (set var * params) := {
-   ParamRel := ParamRel;
-   ArgRel := ArgRel;
-   BlockRel := fun lvZ b b' => True (* F.block_Z b = snd lvZ *)
+(* A proof relation is parameterized by analysis information A *)
+Class ProofRelationI (A:Type) := {
+    (* Relates parameter lists according to analysis information *)
+    ParamRelI : A -> list var -> list var -> Prop;
+    (* Relates argument lists according to analysis information
+       and closure environments *)
+    ArgRelI : onv val -> onv val -> A-> list val -> list val -> Prop;
+    (* Relates blocks according to analysis information *)
+    BlockRelI : A -> I.block -> I.block -> Prop;
+    (* Relates environments according to analysis information *)
+    IndexRelI : 〔A〕 -> nat -> nat -> Prop;
+    ArgLengthMatchI : forall E E' a Z Z' VL VL',
+        ParamRelI a Z Z' -> ArgRelI E E' a VL VL' -> length Z = length VL /\ length Z' = length VL';
+    IndexRelDrop : forall k AL n n', IndexRelI AL n n' -> k <= n -> IndexRelI (drop k AL) (n - k) n'
+(*    IndexRelApp : forall AL AL' n n', IndexRelI AL n n' -> IndexRelI (AL' ++ AL) (❬AL'❭ + n) n' *)
 }.
-intros. inv H; inv H0; simpl in *.
-erewrite filter_filter_by_length; eauto.
-Defined.
+
+Inductive simIBlock (SIM:ProgramEquivalence I.state I.state)
+          (r:I.state -> I.state -> Prop)
+          {A} (AR:ProofRelationI A)
+  : list A -> I.labenv -> I.labenv -> A -> I.block -> I.block -> Prop :=
+| simIBlockI a L L' Z Z' s s' n n' bn' AL
+  : ParamRelI a Z Z'
+    -> BlockRelI a (I.blockI Z s n) (I.blockI Z' s' bn')
+    -> IndexRelI AL n n'
+    -> (forall E E' Yv Y'v Y Y',
+          omap (exp_eval E) Y = Some Yv
+          -> omap (exp_eval E') Y' = Some Y'v
+          -> ArgRelI E E' a Yv Y'v
+          -> progeq r (L, E, stmtApp (LabI n) Y)
+                   (L', E', stmtApp (LabI bn') Y'))
+          -> simIBlock SIM r AR AL L L' a (I.blockI Z s n) (I.blockI Z' s' bn').
 
 
-Lemma agree_on_update_filter X `{OrderedType X} Y `{Equivalence (option Y)}
-      (lv:set X) (V: X -> option Y) Z VL
-: length Z = length VL
-  -> agree_on R lv
-             (V [Z <-- List.map Some VL])
-             (V [List.filter (fun x => B[x ∈ lv]) Z <--
-                             List.map Some (filter_by (fun x => B[x ∈ lv]) Z VL)]).
+Definition renILabenv (SIM:ProgramEquivalence I.state I.state) r
+           {A} AR (AL:list A) L L' :=
+  (length AL = length L /\ sawtooth L' /\ sawtooth L) /\
+  forall n n' a b b', IndexRelI AL n n' -> get AL n a -> get L n b -> get L' n' b'
+               -> simIBlock SIM r AR
+                           (drop (n  - I.block_n b) AL)
+                           (drop (n  - I.block_n b) L)
+                           (drop (n' - I.block_n b') L')
+                           a b b' .
+
+Definition fexteqI (SIM:ProgramEquivalence I.state I.state)
+           {A} (PR:ProofRelationI A) (a:A) (AL:list A) L L' Z s Z' s' :=
+  ParamRelI a Z Z' /\
+  forall E E' VL VL' (r:rel2 I.state (fun _ : I.state => I.state)),
+    ArgRelI E E' a VL VL'
+    -> renILabenv SIM r PR AL L L'
+    -> progeq r (L, E[Z <-- List.map Some VL], s)
+            (L', E'[Z' <-- List.map Some VL'], s').
+
+Lemma sawtooth_get_drop {B} `{BlockType B} L f b
+: sawtooth L
+  -> get L f b
+  -> get (drop (f - block_n b) L) (block_n b) b.
 Proof.
-  intros. eapply length_length_eq in H1.
-  general induction H1.
-  - eapply agree_on_refl. eapply H0.
-  - simpl. cases. simpl. eapply agree_on_update_same. reflexivity.
-    eapply agree_on_incl. eapply IHlength_eq. eauto. cset_tac; intuition.
-    eapply agree_on_update_dead; eauto.
+    intros. general induction H0; simpl; isabsurd.
+    get_cases H2.
+    - exploit tooth_index; eauto.
+      rewrite H3.
+      orewrite (f + 0 = f).
+      orewrite (f - f = 0).
+      simpl. eapply get_app; eauto.
+    - exploit (sawtooth_smaller H0 H2).
+      specialize (IHsawtooth _ _ H2).
+      orewrite (f - block_n b
+                = length L + (f - length L - block_n b)).
+      rewrite drop_app; eauto.
 Qed.
 
-Lemma agree_on_update_filter' X `{OrderedType X} Y `{Equivalence (option Y)} (lv:set X) (V V':X -> option Y) Z VL
-: length Z = length VL
-  -> agree_on R (lv \ of_list Z) V V'
-  -> agree_on R lv
-             (V [Z <-- List.map Some VL])
-             (V' [(List.filter (fun x => B[x ∈ lv]) Z) <-- (List.map Some
-                             (filter_by (fun x => B[x ∈ lv]) Z VL))]).
+Lemma fix_compatible_I r A (PR:ProofRelationI A) (a:A) AL F F' E E' Z Z' L L' Yv Y'v s s' n n' AL' bn
+(LEN2:length AL' = length F)
+  : renILabenv sim_progeq r PR AL L L'
+    -> (forall n n' Z s Z' s' a bn, get F n (Z,s) -> IndexRelI (AL' ++ AL) n n'
+                              -> get (mapi I.mkBlock F' ++ L') n' (I.blockI Z' s' bn) -> get AL' n a ->
+                              fexteqI sim_progeq PR a
+                                      (AL' ++ AL)
+                                      (mapi I.mkBlock F ++ L)
+                                      (mapi I.mkBlock F' ++ L') Z s Z' s'
+                              /\ BlockRelI a (I.blockI Z s n) (I.blockI Z' s' bn)
+                              /\ ParamRelI a Z Z')
+    -> get F n (Z,s)
+    -> IndexRelI (AL' ++ AL) n n'
+    -> get (mapi I.mkBlock F' ++ L') n' (I.blockI Z' s' bn)
+    -> get AL' n a
+    -> ArgRelI E E' a Yv Y'v
+    -> sim'r r
+              (mapi I.mkBlock F ++ L, E [Z <-- List.map Some Yv], s)
+              (mapi I.mkBlock F' ++ L', E' [Z' <-- List.map Some Y'v], s').
 Proof.
-  intros.
-  eapply agree_on_trans. eapply H0.
-  eapply update_with_list_agree; eauto. rewrite map_length; eauto.
-  eapply agree_on_update_filter; eauto.
+  revert_all; pcofix CIH; intros.
+  eapply H1; eauto. clear H2 H3 H4 H5 H6. clear s s' Z Z' n n' a bn.
+  hnf. split.
+  destruct H0; dcr; split; eauto with len. split; eauto.
+  econstructor; eauto. eapply tooth_I_mkBlocks.
+  econstructor; eauto. eapply tooth_I_mkBlocks.
+  intros ? ? ? ? ? RN GetAL GetFL GetL'.
+  assert (❬AL'❭ = ❬mapi I.mkBlock F❭) by eauto with len.
+  eapply get_app_cases in GetAL. destruct GetAL.
+  - eapply get_app_lt_1 in GetFL; [| rewrite <- H; eauto using get_range].
+    inv_get. destruct x as [Z s]. destruct b' as [Z' s' bn]. simpl.
+    orewrite (n - n = 0). simpl.
+    exploit H1; eauto; dcr.
+    eapply simIBlockI; eauto. simpl.
+    intros.
+    exploit (ArgLengthMatchI); eauto; dcr.
+    exploit (omap_length _ _ _ _ _ H3).
+    exploit (omap_length _ _ _ _ _ H5).
+    pone_step; eauto using get_app, get_mapi; eauto; simpl.
+    congruence. assert (sawtooth (mapi I.mkBlock F' ++ L')).
+    econstructor. eapply H0. eapply tooth_I_mkBlocks.
+    eapply (sawtooth_get_drop H13 GetL'). simpl. omega.
+    right. simpl.
+    orewrite (n - n = 0); simpl.
+    orewrite (bn - bn = 0); simpl.
+    eapply CIH; eauto.
+  - destruct H0.
+    dcr. eapply get_app_right_ge in GetFL; [ | rewrite <- H; eauto].
+    assert (n - I.block_n b >= ❬mapi I.mkBlock F❭). {
+      exploit (sawtooth_smaller H8 GetFL). rewrite <- H in *. simpl in *. omega.
+    }
+    exploit H3. instantiate (2:=n-❬mapi I.mkBlock F❭). instantiate (1:=n').
+    eapply IndexRelDrop in RN. instantiate (1:=❬AL'❭) in RN.
+    rewrite drop_length_eq in RN. rewrite <- H. eauto. omega.
+    rewrite <- H. eauto. eauto. eauto.
+    rewrite (drop_app_gen _ (mapi I.mkBlock F)); eauto.
+    assert (EQ:n - ❬mapi I.mkBlock F❭ - I.block_n b = n - I.block_n b - ❬mapi I.mkBlock F❭)
+      by omega.
+    rewrite <- EQ.
+    inv H6. econstructor; eauto. simpl in *.
+    rewrite (drop_app_gen _ AL'); eauto.
+    rewrite H. rewrite <- EQ. eauto. omega.
+    intros. eapply progeq_mon; eauto.
 Qed.
 
 
-Lemma sim_DVE' r L L' V V' s LV lv
-: agree_on eq (getAnn lv) V V'
--> true_live_sound Functional LV s lv
--> simL' sim_progeq r SR LV L L'
--> sim'r r (L,V, s) (L',V', compile LV s lv).
+Lemma renILabenv_extension r A (PR:ProofRelationI A) (AL AL':list A) F F' L L'
+      (LEN1:length AL' = length F)
+  : renILabenv sim_progeq r PR AL L L'
+    -> (forall n n' Z s Z' s' a bn, get F n (Z,s) -> IndexRelI (AL' ++ AL) n n'
+                              -> get (mapi I.mkBlock F' ++ L') n' (I.blockI Z' s' bn) -> get AL' n a ->
+                              fexteqI sim_progeq PR a
+                                      (AL' ++ AL)
+                                      (mapi I.mkBlock F ++ L)
+                                      (mapi I.mkBlock F ++ L') Z s Z' s'
+                              /\ BlockRelI a (I.blockI Z s n) (I.blockI Z' s' bn)
+                              /\ ParamRelI a Z Z')
+  -> renILabenv sim_progeq r PR (AL' ++ AL) (mapi I.mkBlock F ++ L) (mapi I.mkBlock F' ++ L').
 Proof.
-  unfold simL', sim'r. revert_except s.
-  sind s; destruct s; simpl; intros; invt true_live_sound; simpl in * |- *.
-  - case_eq (exp_eval V e); intros. cases.
-    + pone_step.
-      instantiate (1:=v). erewrite exp_eval_live; eauto. eapply agree_on_sym; eauto.
-      left. eapply (IH s); eauto. eapply agree_on_update_same; eauto with cset.
-    + eapply sim'_expansion_closed;
-      [ | eapply S_star2 with (y:=EvtTau);
-          [ econstructor; eauto | eapply star2_refl ]
-        | eapply star2_refl].
-      eapply (IH s); eauto. eapply agree_on_update_dead; eauto with cset.
-    + pfold. econstructor 3; [| eapply star2_refl|]; eauto. stuck.
-  - repeat cases.
-    + edestruct (exp2bool_val2bool V); eauto; dcr.
-      eapply sim'_expansion_closed.
-      eapply (IH s1); eauto. eapply agree_on_incl; eauto.
-      eapply H10; congruence.
-      eapply S_star2 with (y:=EvtTau) (yl:=nil).
-      econstructor; eauto. eapply star2_refl.
-      eapply star2_refl.
-    + edestruct (exp2bool_val2bool V); eauto; dcr.
-      eapply sim'_expansion_closed.
-      eapply (IH s2); eauto. eapply agree_on_incl; eauto.
-      eapply S_star2 with (y:=EvtTau) (yl:=nil).
-      econstructor 3; eauto. eapply star2_refl.
-      eapply star2_refl.
-    + remember (exp_eval V e). symmetry in Heqo.
-      exploit exp_eval_live_agree; eauto.
-      eapply H8. case_eq (exp2bool e); intros; try destruct b; congruence.
-      destruct o. case_eq (val2bool v); intros.
-      pone_step. left. eapply IH; eauto with cset.
-      pone_step. left; eapply (IH s2); eauto with cset.
-      pno_step.
-  - destruct (get_dec L (counted l)) as [[[bE bZ bs]]|].
-    + remember (omap (exp_eval V) Y). symmetry in Heqo.
-      rewrite (get_nth (∅, nil) H4); simpl.
-      destruct o.
-      * exploit omap_filter_by; eauto.
-        unfold simL' in H1. inRel_invs. simpl in *.
-        hnf in H17; dcr; subst; simpl in *.
-        eapply sim_drop_shift; eauto.
-        eapply (inRel_sawtooth H1). eapply (inRel_sawtooth H1). eapply H19. eauto.
-        eapply omap_exp_eval_live_agree; eauto.
-        eapply argsLive_liveSound; eauto.
-        hnf; split; eauto. simpl. exploit omap_length; try eapply Heqo; eauto.
-        congruence.
-      * pfold; econstructor 3; try eapply star2_refl; eauto; stuck2.
-    + pfold; econstructor 3; try eapply star2_refl; eauto; stuck2.
-  - pno_step; simpl. erewrite <- exp_eval_live_agree; eauto; symmetry; eauto.
-  - remember (omap (exp_eval V) Y). symmetry in Heqo.
-    exploit omap_exp_eval_live_agree; eauto.
-    destruct o.
-    + pextern_step; eauto using agree_on_update_same, agree_on_incl; try congruence.
-    + pno_step.
-  - pone_step. left. eapply IH; eauto with cset.
-    + eapply simL_mon; eauto. eapply simL_extension'; eauto with len.
-      * intros. inv_get; simpl. split. hnf; intros; simpl.
-        unfold ParamRel, ArgRel. intuition.
-        eapply (IH s1); eauto. subst.
-        eapply agree_on_update_filter'; eauto.
-        eapply agree_on_incl; eauto. simpl.
-        exploit H8; eauto.
-        exploit H6; eauto.
-        unfold ParamRel. intuition.
-Qed.
-
-Lemma sim_DVE V V' s lv
-: agree_on eq (getAnn lv) V V'
--> true_live_sound Functional nil s lv
--> @sim F.state _ F.state _ (nil,V, s) (nil,V', compile nil s lv).
-Proof.
-  intros. eapply sim'_sim.
-  eapply sim_DVE'; eauto. hnf. econstructor.
+  intros. destruct H.
+  split. dcr. split. eauto with len.
+  split; eauto.
+  econstructor; eauto using tooth_I_mkBlocks.
+  econstructor; eauto using tooth_I_mkBlocks.
+  intros ? ? ? ? ? RN GetAL GetL GetL'.
+  assert (ALLEN:❬AL'❭ = ❬mapi I.mkBlock F❭) by eauto with len.
+  eapply get_app_cases in GetAL. destruct GetAL.
+  - eapply get_app_lt_1 in GetL; [| rewrite <- ALLEN; eauto using get_range].
+    inv_get. destruct x, b'.
+    exploit H0; eauto. simpl in *. dcr.
+    destruct H4. orewrite (n - n = 0); simpl.
+    econstructor; eauto. intros.
+    exploit (ArgLengthMatchI); eauto; dcr.
+    exploit (omap_length _ _ _ _ _ H5).
+    exploit (omap_length _ _ _ _ _ H10).
+    pone_step; eauto using get_app, get_mapi; simpl; eauto with len.
+    left. orewrite (n - n = 0); simpl.
+    exploit (tooth_index H8 GetL'); eauto. simpl in *.
+    orewrite (n' + 0 = n') in H16. subst; simpl in *.
+    orewrite (n' - n' = 0); simpl.
+    eapply fix_compatible_I; eauto.
+    split; eauto.
+  - dcr.
+    eapply get_app_right_ge in GetL; [ | rewrite <- ALLEN; eauto].
+    assert (n - I.block_n b >= ❬mapi I.mkBlock F❭). {
+      exploit (sawtooth_smaller H7 GetL). rewrite <- ALLEN in *. simpl in *. omega.
+    }
+    rewrite (drop_app_gen _ (mapi I.mkBlock F)); eauto.
+    rewrite (drop_app_gen _ AL'); [ | rewrite ALLEN; eauto ].
+    assert (EQ:n - ❬mapi I.mkBlock F❭ - I.block_n b = n - I.block_n b - ❬mapi I.mkBlock F❭)
+      by omega.
+    rewrite ALLEN. rewrite <- EQ.
+    eapply H1; eauto.
+    eapply IndexRelDrop in RN. instantiate (1:= ❬mapi I.mkBlock F❭) in RN.
+    rewrite <- ALLEN in RN. rewrite drop_length_eq in RN.
+    rewrite ALLEN in RN. eauto. rewrite <- ALLEN. omega.
+    rewrite <- ALLEN. eauto.
 Qed.
 
 Module I.
 
   Require Import SimI.
 
-Definition ArgRel (V V':onv val) (G:(set var * params)) (VL VL': list val) : Prop :=
-  VL' = (filter_by (fun x => B[x ∈ (fst G)]) (snd G) VL) /\
-  length (snd G) = length VL /\
-  agree_on eq (fst G \ of_list (snd G)) V V'.
+  Definition ArgRel (V V':onv val) (G:؟(set var) * params) (VL VL': list val) : Prop :=
+      VL' = (filter_by (fun x => B[x ∈ oget (fst G)]) (snd G) VL) /\
+      length (snd G) = length VL /\
+      agree_on eq (oget (fst G) \ of_list (snd G)) V V'.
 
-Definition ParamRel (G:(set var * params)) (Z Z' : list var) : Prop :=
-  Z' = (List.filter (fun x => B[x ∈ (fst G)]) Z) /\ snd G = Z.
 
-Instance SR : ProofRelationI (set var * params) := {
+  Definition ParamRel (G:option (set var) * params) (Z Z' : list var) : Prop :=
+    Z' = (List.filter (fun x => B[x ∈ oget (fst G)]) Z) /\ snd G = Z.
+
+Instance SR : ProofRelationI (؟(set var) * params) := {
    ParamRelI := ParamRel;
    ArgRelI := ArgRel;
-   BlockRelI := fun lvZ b b' => I.block_Z b = snd lvZ
+   BlockRelI := fun lvZ b b' => True;
+   IndexRelI a b c := True
 }.
-intros. inv H; inv H0; dcr; simpl in *.
+intros. hnf in H, H0; dcr; subst.
 erewrite filter_filter_by_length; eauto.
-Defined.
+intros. admit.
+Admitted.
 
 Lemma sim_I r L L' V V' s LV lv
-: agree_on eq (getAnn lv) V V'
+: agree_on eq (getOAnn lv) V V'
 -> true_live_sound Imperative LV s lv
--> simILabenv sim_progeq r SR LV L L'
+-> renILabenv sim_progeq r SR LV L L'
 -> sim'r r (L,V, s) (L',V', compile LV s lv).
 Proof.
-  unfold simILabenv, sim'r. revert_except s.
+  unfold sim'r. revert_except s.
   sind s; destruct s; simpl; intros; invt true_live_sound; simpl in * |- *.
-  - case_eq (exp_eval V e); intros. cases.
-    + pone_step. instantiate (1:=v).
-      erewrite exp_eval_live; eauto. eapply agree_on_sym; eauto.
-      left. eapply (IH s); eauto. eapply agree_on_update_same. reflexivity.
-      eapply agree_on_incl; eauto.
-    + eapply sim'_expansion_closed;
-      [ | eapply S_star2 with (y:=EvtTau);
-          [ econstructor; eauto | eapply star2_refl ]
-        | eapply star2_refl].
-      eapply (IH s); eauto. eapply agree_on_update_dead; eauto.
-      eapply agree_on_incl; eauto. rewrite <- H9. cset_tac; intuition.
+  - case_eq (exp_eval V e); intros.
+    + cases.
+      *  pone_step. instantiate (1:=v).
+         erewrite exp_eval_live; eauto. eapply agree_on_sym; eauto.
+         left. eapply (IH s); eauto. eapply agree_on_update_same. reflexivity.
+         eapply agree_on_incl; eauto.
+      *  eapply sim'_expansion_closed;
+           [ | eapply S_star2 with (y:=EvtTau);
+               [ econstructor; eauto | eapply star2_refl ]
+             | eapply star2_refl].
+         eapply (IH s); eauto. eapply agree_on_update_dead; eauto.
+         eapply agree_on_incl; eauto. rewrite <- H9. cset_tac; intuition.
     + pfold. econstructor 3; [| eapply star2_refl|]; eauto. stuck.
   - repeat cases.
     + edestruct (exp2bool_val2bool V); eauto; dcr.
@@ -233,10 +300,10 @@ Proof.
       stuck.
   - destruct (get_dec L (counted l)) as [[[bZ bs]]|].
     + remember (omap (exp_eval V) Y). symmetry in Heqo.
-      rewrite (get_nth (∅, nil) H4); eauto; simpl.
+      rewrite (get_nth (None, nil) H4); eauto; simpl.
       destruct o.
       * exploit omap_filter_by; eauto.
-        hnf in H1. inRel_invs; simpl in *; subst.
+        (*hnf in H1; dcr. exploit H6; eauto.
         hnf in H15. dcr; simpl in *; clear_trivial_eqs; subst.
         eapply sim_drop_shift_I. eapply (inRel_sawtooth H1).
         eapply (inRel_sawtooth H1). eauto. eauto.
@@ -246,7 +313,8 @@ Proof.
         eapply argsLive_liveSound; eauto.
         hnf; split; eauto. simpl. split.
         exploit omap_length; try eapply Heqo; eauto. congruence.
-        eapply agree_on_incl; eauto.
+        eapply agree_on_incl; eauto.*)
+        admit.
       * pfold; econstructor 3; try eapply star2_refl; eauto; stuck2.
     + pfold; econstructor 3; try eapply star2_refl; eauto; stuck2.
   - pno_step.
@@ -258,7 +326,7 @@ Proof.
     + pno_step.
   - pone_step. left. eapply IH; eauto.
     + simpl in *; eapply agree_on_incl; eauto.
-    + eapply simILabenv_mon; eauto. eapply simILabenv_extension; eauto with len.
+    + eapply renILabenv_extension.
       * intros. inv_get; simpl. split. hnf; intros; simpl.
         unfold ParamRel, ArgRel. intuition.
         eapply (IH s1); eauto. subst.
@@ -277,6 +345,31 @@ Proof.
 Qed.
 
 End I.
+
+
+Definition ArgRel (V V:onv val) (G:option (set var * params)) (VL VL': list val) : Prop :=
+  match G with
+  | Some G => VL' = (filter_by (fun x => B[x ∈ (fst G)]) (snd G) VL) /\ length (snd G) = length VL
+  | None => VL' = VL
+  end.
+
+Definition ParamRel (G:(؟(set var * params))) (Z Z' : list var) : Prop :=
+  match G with
+  | Some G => Z' = (List.filter (fun x => B[x ∈ (fst G)]) Z) /\ snd G = Z
+  | None => True
+  end.
+
+Instance SR : ProofRelationI (؟(set var * params)) :=
+  {
+    ParamRelI := ParamRel;
+    ArgRelI := ArgRel;
+    BlockRelI := fun lvZ b b' => True;
+    IndexRelI D n n' := True
+  }.
+Proof.
+intros. hnf in H, H0. destruct a; dcr. subst.
+erewrite filter_filter_by_length; eauto.
+Admitted.
 
 
 Fixpoint compile_live (s:stmt) (a:ann (set var)) (G:set var) : ann (set var) :=
@@ -401,4 +494,85 @@ Proof.
       rewrite of_list_filter.
       clear_all; cset_tac.
     + rewrite compile_live_incl; eauto with cset.
+Qed.
+
+Lemma sim_DVE' r L L' V V' s LV lv
+: agree_on eq (getAnn lv) V V'
+-> true_live_sound Functional LV s lv
+-> simL' sim_progeq r SR LV L L'
+-> sim'r r (L,V, s) (L',V', compile LV s lv).
+Proof.
+  unfold simL', sim'r. revert_except s.
+  sind s; destruct s; simpl; intros; invt true_live_sound; simpl in * |- *.
+  - case_eq (exp_eval V e); intros. cases.
+    + pone_step.
+      instantiate (1:=v). erewrite exp_eval_live; eauto. eapply agree_on_sym; eauto.
+      left. eapply (IH s); eauto. eapply agree_on_update_same; eauto with cset.
+    + eapply sim'_expansion_closed;
+      [ | eapply S_star2 with (y:=EvtTau);
+          [ econstructor; eauto | eapply star2_refl ]
+        | eapply star2_refl].
+      eapply (IH s); eauto. eapply agree_on_update_dead; eauto with cset.
+    + pfold. econstructor 3; [| eapply star2_refl|]; eauto. stuck.
+  - repeat cases.
+    + edestruct (exp2bool_val2bool V); eauto; dcr.
+      eapply sim'_expansion_closed.
+      eapply (IH s1); eauto. eapply agree_on_incl; eauto.
+      eapply H10; congruence.
+      eapply S_star2 with (y:=EvtTau) (yl:=nil).
+      econstructor; eauto. eapply star2_refl.
+      eapply star2_refl.
+    + edestruct (exp2bool_val2bool V); eauto; dcr.
+      eapply sim'_expansion_closed.
+      eapply (IH s2); eauto. eapply agree_on_incl; eauto.
+      eapply S_star2 with (y:=EvtTau) (yl:=nil).
+      econstructor 3; eauto. eapply star2_refl.
+      eapply star2_refl.
+    + remember (exp_eval V e). symmetry in Heqo.
+      exploit exp_eval_live_agree; eauto.
+      eapply H8. case_eq (exp2bool e); intros; try destruct b; congruence.
+      destruct o. case_eq (val2bool v); intros.
+      pone_step. left. eapply IH; eauto with cset.
+      pone_step. left; eapply (IH s2); eauto with cset.
+      pno_step.
+  - destruct (get_dec L (counted l)) as [[[bE bZ bs]]|].
+    + remember (omap (exp_eval V) Y). symmetry in Heqo.
+      rewrite (get_nth (∅, nil) H4); simpl.
+      destruct o.
+      * exploit omap_filter_by; eauto.
+        unfold simL' in H1. inRel_invs. simpl in *.
+        hnf in H17; dcr; subst; simpl in *.
+        eapply sim_drop_shift; eauto.
+        eapply (inRel_sawtooth H1). eapply (inRel_sawtooth H1). eapply H19. eauto.
+        eapply omap_exp_eval_live_agree; eauto.
+        eapply argsLive_liveSound; eauto.
+        hnf; split; eauto. simpl. exploit omap_length; try eapply Heqo; eauto.
+        congruence.
+      * pfold; econstructor 3; try eapply star2_refl; eauto; stuck2.
+    + pfold; econstructor 3; try eapply star2_refl; eauto; stuck2.
+  - pno_step; simpl. erewrite <- exp_eval_live_agree; eauto; symmetry; eauto.
+  - remember (omap (exp_eval V) Y). symmetry in Heqo.
+    exploit omap_exp_eval_live_agree; eauto.
+    destruct o.
+    + pextern_step; eauto using agree_on_update_same, agree_on_incl; try congruence.
+    + pno_step.
+  - pone_step. left. eapply IH; eauto with cset.
+    + eapply simL_mon; eauto. eapply simL_extension'; eauto with len.
+      * intros. inv_get; simpl. split. hnf; intros; simpl.
+        unfold ParamRel, ArgRel. intuition.
+        eapply (IH s1); eauto. subst.
+        eapply agree_on_update_filter'; eauto.
+        eapply agree_on_incl; eauto. simpl.
+        exploit H8; eauto.
+        exploit H6; eauto.
+        unfold ParamRel. intuition.
+Qed.
+
+Lemma sim_DVE V V' s lv
+: agree_on eq (getAnn lv) V V'
+-> true_live_sound Functional nil s lv
+-> @sim F.state _ F.state _ (nil,V, s) (nil,V', compile nil s lv).
+Proof.
+  intros. eapply sim'_sim.
+  eapply sim_DVE'; eauto. hnf. econstructor.
 Qed.
